deps/poulet4/lib/P4cub/Syntax/Shift.v
@@ -7,53 +7,58 @@ Local Open Scope expr_scope.
 
 (** * Philip Wadler style de Bruijn shifts for expression variables. *)
 
-Definition ext (ρ : nat -> nat) (x : nat) :=
-  match x with
-  | O   => O
-  | S n => S $ ρ x
-  end.
+Section Rename.
+  Variable ρ : nat -> nat.
 
-Fixpoint rename_e (ρ : nat -> nat) (e : Expr.e) : Expr.e :=
-  match e with
-  | Expr.Bool _
-  | _ `W _
-  | _ `S _
-  | Expr.Error _     => e
-  | Expr.Var t x     => Expr.Var t $ ρ x
-  | Expr.Slice e h l => Expr.Slice (rename_e ρ e) h l
-  | Expr.Cast t e    => Expr.Cast t $ rename_e ρ e
-  | Expr.Uop t op e  => Expr.Uop t op $ rename_e ρ e
-  | Expr.Member t x e
-    => Expr.Member t x $ rename_e ρ e
-  | Expr.Bop t op e1 e2
-    => Expr.Bop t op (rename_e ρ e1) (rename_e ρ e2)
-  | Expr.Struct es ob
-    => Expr.Struct (map (rename_e ρ) es) ob
-  end.
+  Definition ext (x : nat) :=
+    match x with
+    | O   => O
+    | S n => S $ ρ x
+    end.
 
-Local Close Scope expr_scope.
+  Fixpoint rename_e  (e : Expr.e) : Expr.e :=
+    match e with
+    | Expr.Bool _
+    | _ `W _
+    | _ `S _
+    | Expr.Error _     => e
+    | Expr.Var t x     => Expr.Var t $ ρ x
+    | Expr.Slice h l e => Expr.Slice h l $ rename_e e
+    | Expr.Cast t e    => Expr.Cast t $ rename_e e
+    | Expr.Uop t op e  => Expr.Uop t op $ rename_e e
+    | Expr.Index t e1 e2
+      => Expr.Index t (rename_e e1) $ rename_e e2
+    | Expr.Member t x e
+      => Expr.Member t x $ rename_e e
+    | Expr.Bop t op e1 e2
+      => Expr.Bop t op (rename_e e1) $ rename_e e2
+    | Expr.Lists l es => Expr.Lists l $ map rename_e es
+    end.
+  
+  Local Close Scope expr_scope.
 
-Definition rename_arg (ρ : nat -> nat)
-  : paramarg Expr.e Expr.e -> paramarg Expr.e Expr.e :=
-  paramarg_map_same $ rename_e ρ.
+  Definition rename_arg
+    : paramarg Expr.e Expr.e -> paramarg Expr.e Expr.e :=
+    paramarg_map_same $ rename_e.
 
-Definition rename_fun_kind (ρ : nat -> nat) (fk : Stmt.fun_kind)
-  : Stmt.fun_kind :=
-  match fk with
-  | Stmt.Funct f τs oe
-    => Stmt.Funct f τs $ option_map (rename_e ρ) oe
-  | Stmt.Action a cargs
-    => Stmt.Action a $ map (rename_e ρ) cargs
-  | Stmt.Method e m τs oe
-    => Stmt.Method e m τs $ option_map (rename_e ρ) oe
-  end.
+  Definition rename_fun_kind (fk : Stmt.fun_kind)
+    : Stmt.fun_kind :=
+    match fk with
+    | Stmt.Funct f τs oe
+      => Stmt.Funct f τs $ option_map rename_e oe
+    | Stmt.Action a cargs
+      => Stmt.Action a $ map rename_e cargs
+    | Stmt.Method e m τs oe
+      => Stmt.Method e m τs $ option_map rename_e oe
+    end.
 
-Definition rename_transition (ρ : nat -> nat) (e : Parser.e) : Parser.e :=
-  match e with
-  | Parser.Goto _ => e
-  | Parser.Select e d cases
-    => Parser.Select (rename_e ρ e) d cases
-  end.
+  Definition rename_transition (e : Parser.e) : Parser.e :=
+    match e with
+    | Parser.Direct _ => e
+    | Parser.Select e d cases
+      => Parser.Select (rename_e e) d cases
+    end.
+End Rename.
 
 Local Open Scope stmt_scope.
 
